theories/Tester.v
@@ -173,60 +173,20 @@ Definition instantiate_observe {E A} `{Is__stE E} (e : observeE A)
       Ret (s, pkt)
     end.
 
-Definition liftState {S A} {F : Type -> Type} `{Functor F} (aF : F A)
-  : Monads.stateT S F A :=
-  fun s : S => pair s <$> aF.
-
 Definition unifier {E R} `{Is__stE E} (m : itree oE R)
   : Monads.stateT unify_state (itree E) R :=
   interp (fun _ e =>
             match e with
             | (|||ue|)  => instantiate_unify   ue
             | (|||||oe) => instantiate_observe oe
-            | (e|)
+            | (Throw err|) =>
+              fun s =>
+                embed Log ("Failing state: " ++ to_string s);;
+                throw err
             | (|e|)
             | (||e|)
             | (||||e|) => @liftState unify_state _ (itree _) _ (trigger e)
             end) m.
-
-Variant traceT :=
-  Trace__In  : packetT id -> traceT
-| Trace__Out : packetT id -> traceT.
-
-Instance Serialize__traceT : Serialize traceT :=
-  fun t =>
-    match t with
-    | Trace__In  p => [Atom "In";  to_sexp p]
-    | Trace__Out p => [Atom "Out"; to_sexp p]
-    end%sexp.
-
-Definition list_to_string {A} `{Serialize A} (l : list A) : string :=
-  String.concat CRLF (map to_string l).
-
-Definition logger {E R} `{Is__stE E} (m : itree stE R)
-  : Monads.stateT (list traceT) (itree E) R :=
-  interp
-    (fun _ e =>
-       match e with
-       | (Throw err|) =>
-         fun s =>
-           embed Log ("Failing trace: " ++ CRLF ++ list_to_string (rev' s));;
-           throw err
-       | (||||e) =>
-         match e in testerE Y return Monads.stateT _ _ Y with
-         | Tester__Recv c =>
-           fun s =>
-             pkt <- embed Tester__Recv c;;
-             ret (Trace__In pkt::s, pkt)
-         | Tester__Send ss c es =>
-           fun s =>
-             pkt <- embed Tester__Send ss c es;;
-             ret (Trace__Out pkt::s, pkt)
-         end
-       | (|e|)
-       | (||e|)
-       | (|||e|) => @liftState (list traceT) _ (itree _) _ (trigger e)
-       end) m.
 
 CoFixpoint match_event {T R} (e0 : testerE R) (r : R) (m : itree stE T)
   : itree stE T :=
@@ -321,5 +281,5 @@ CoFixpoint backtrack' {E R} `{Is__tE E} (others : list (itree stE R))
 Definition backtrack {E R} `{Is__tE E} : itree stE R -> itree E R :=
   backtrack' [].
 
-Definition tester {E R} `{Is__tE E} (mo : itree oE R) :=
-  backtrack $ logger (unifier mo (0, [], [], [])) [].
+Definition tester {E R} `{Is__tE E} (mo : itree oE R) : itree E R :=
+  backtrack $ snd <$> unifier mo (0, [], [], []).
